Pass over all lectures

src/syntax1.dfy
@@ -1,17 +1,12 @@
 /* Mathematical reasoning in Dafny */
 
-/* Outline:
-- Assertion
-- Functions
-- Lemmas
-*/
+/*** Mathematical assertions ***/
 
-/** Mathematical assertions **/
-
-/* A lemma can contain assertions. Unlike programming assertions, Dafny will
-statically check each assertion and report an error if it cannot prove it. This
-is similar to how the compiler checks your types and reports an error if they
-don't match. */
+/* The first bit of Dafny we introduce is the lemma and assertions. A lemma is
+ * like a method or procedure in other languages. Unlike in other languages,
+ * Dafny will statically check each assertion in a lemma and report an error if
+ * it cannot prove it. This is similar to how the compiler checks your types and
+ * reports an error if they don't match. */
 
 lemma SomeAssertions() {
   assert 2 + 2 == 4;
@@ -21,24 +16,31 @@ lemma SomeAssertions() {
   assert 1 + 2*3 == 7;
 }
 
-lemma BooleanFacts() {
+/* Here are a few more built-in Dafny operators, which are used for stating logical facts: */
+
+lemma LogicalOperators() {
+  assert true && (true || false);
   assert true == false || true;
   // Dafny has a boolean implies operator written p ==> q. As you might recall,
   // p ==> q is the same as !p || q. Implications are quite common when writing
   // logical properties.
   assert !(true ==> false);
   assert false ==> false;
+  // Dafny also has a boolean "if and only if" operator. This is identical to ==
+  // for booleans, but it often conveys intent better when used for assertions.
+  assert false <==> false;
+  assert !(true <==> false);
 }
 
 
 
 /*** Functions ***/
 
-/* A Dafny `function` is a mathematical function: it is always deterministic,
-and is written without mutable variables or data structures. Functions are one
-way to build interesting objects to prove things about in Dafy. In the next
-lecture we'll see datatypes (both built-in and user-defined) which will give us
-a lot more to play with. */
+/* A Dafny `function` is a mathematical function: it is always deterministic, and
+ * is written without mutable variables or data structures. Functions are one way
+ * to define something interesting to prove properties about in Dafy. In the next
+ * lecture we'll see datatypes (both built-in and user-defined) which will give
+ * us a lot more to play with. */
 
 function Enlargen(x: int): int {
   2 * x + 5
@@ -48,7 +50,14 @@ function IsLarge(x: int): bool {
   x > 1000
 }
 
-function LocalVars(b: bool, i1: int, i2: int): bool {
+// New syntax (predicate): `predicate` is a shorthand for a function that returns a boolean.
+// Functions that return a boolean are extremely common in verification since
+// they express logical predicates, hence the special syntax.
+predicate IsSmall(x: int) {
+  !IsLarge(x)
+}
+
+predicate LocalVars(b: bool, i1: int, i2: int) {
   // we can create (immutable) local variables to break up large function
   // definitions
   var larger := i1 > i2;
@@ -56,9 +65,12 @@ function LocalVars(b: bool, i1: int, i2: int): bool {
 }
 
 function abs(x: int): int {
-  /* if is an _expression_ in Dafny, not a _statement_ */
+  // In a function, `if` is an _expression_ in Dafny. We'll see `if`
+  // _statements_ in lemmas later.
   if x < 0 then -x else x
 }
+
+
 
 /*** Lemmas ***/
 
@@ -91,16 +103,18 @@ lemma AbsStrictlyLarger_attempt(x: int)
 }
 
 /* Based on what we learned in the proof of AbsStrictlyLarger, here's a lemma
- that does verify. */
+ * that does verify. */
 
 lemma AbsNegLarger(x: int)
   requires x < 0
   ensures abs(x) > x
 {}
 
-/* The body of a lemma is only used to prove the postcondition; outside of the
- * body, the only thing Dafny will use about a lemma (for example, when it is
- * called) is its precondition and postcondition. */
+/* The statement of a lemma (its pre- and post-condition) is an _abstraction
+ * boundary_ in Dafny that divides the body from the "outside world" (all the
+ * code that uses the lemma). The body of a lemma is used to prove its
+ * postcondition, assuming its precondition; outside of the body, Dafny will
+ * ignore the body.  */
 
 
 
@@ -112,6 +126,10 @@ lemma AbsNegLarger(x: int)
 
 lemma ForallAssertionExamples()
 {
+  // These assertions are different from what we'd normally have in a
+  // programming language because they aren't _executable_. These are
+  // mathematical assertions that can be checked statically, but not by simply
+  // running them since they talk about all integers.
   assert forall x: int :: x + 1 > x;
   assert forall x: int, y: int :: x + y == y + x;
   assert forall b: bool :: b || !b;
@@ -122,13 +140,13 @@ lemma ForallAssertionExamples()
 lemma AbsLargerForAll()
   ensures forall x: int :: abs(x) >= x
 {
-  /* This is a bit of new syntax: a _forall statement_ allows us to help Dafny
-   * with a proof of `forall x` by talking about an individual x */
+  // New syntax (forall statement): a _forall statement_ allows us to help Dafny with a proof of
+  // `forall x :: ...` by talking about an individual `x` */
   forall x: int
     ensures abs(x) >= x
   {
     // Within the body of a forall statement, the proof can refer to `x` when
-    // proving the ensures clause, which means // we can call lemmas, do `if` case
+    // proving the ensures clause, which means we can call lemmas, do `if` case
     // splits, etc.
     AbsLarger(x);
   }
